theories/Native_Development_Machinery.thy
@@ -1,0 +1,10 @@
+theory Native_Development_Machinery
+  imports Development_Machinery Native_Execution_Refinements
+begin
+
+export_code development_seed_report_value development_machinery_state
+  development_machinery_problem_value development_machinery_loop_value development_machinery_unanswered
+  finite_term_shared_word_fold
+  in Eval module_name Native_Development_Machinery file_prefix "native_development_machinery"
+
+end
